SI resources trace proof

aneris/examples/transactional_consistency/implication_trace_util.v
@@ -290,8 +290,8 @@ Section trace_proof_util.
         ([∗ set] sa ∈ clients, client_trace_state_resources lt T sa γmstate γmname extract mstate mname).
 
   Definition GlobalInvExt (test : commitTest) (T : list transaction) (extract : val → option val) 
-    (γmstate γmlin γmpost γmname γl : gname) (clients : gset socket_address) : iProp Σ := 
-    ∃ t lt exec, trace_is t ∗ OwnLinTrace γl lt ∗ ⌜lin_trace_of lt t⌝ ∗ ⌜∀ t, t ∈ T → t ≠ []⌝ ∗
+    (γmstate γmlin γmpost γmname γl : gname) (clients : gset socket_address) (exec : execution) : iProp Σ := 
+    ∃ t lt, trace_is t ∗ OwnLinTrace γl lt ∗ ⌜lin_trace_of lt t⌝ ∗ ⌜∀ t, t ∈ T → t ≠ []⌝ ∗
       ⌜extraction_of lt T⌝ ∗ ⌜valid_transactions T⌝ ∗ ⌜valid_sequence lt⌝ ∗
       ⌜based_on exec (comTrans T)⌝ ∗ ⌜valid_execution test exec⌝ ∗
       trace_state_resources lt T γmstate γmname clients extract ∗
