aneris/examples/transactional_consistency/read_uncommitted/trace/implication_trace.v
@@ -21,7 +21,7 @@ Section trace_proof.
   `(res : !RU_resources Mdl Σ) : RU_resources Mdl Σ :=
     {|
       GlobalInv := (GlobalInv ∗ trace_inv trace_inv_name valid_trace_ru ∗ 
-                    inv KVS_InvName (∃ T, GlobalInvExt commit_test_ru T extract γmstate γmlin γmpost γmname γl clients))%I;
+                    inv KVS_InvName (∃ T exec, GlobalInvExt commit_test_ru T extract γmstate γmlin γmpost γmname γl clients exec))%I;
       OwnMemKey k V := (OwnMemKey k V  ∗ (∀ v, ⌜v ∈ V⌝ → ∃ lh tag c, OwnLinHist γl lh ∗ 
                         ⌜(#(LitString tag), (c, (#"WrLin", (#(LitString k), v))))%V ∈ lh⌝))%I;
       OwnLocalKey k c ov := (OwnLocalKey k c ov ∗ ∃ (sa : socket_address) (γ : gname), ghost_map_elem γmname sa DfracDiscarded (γ, c) ∗ 
@@ -75,7 +75,7 @@ Section trace_proof.
   (lib : KVS_transaction_api) : 
     ⌜KVS_InvName = nroot .@ "kvs_inv"⌝ -∗
     trace_inv trace_inv_name valid_trace_ru -∗
-    inv KVS_InvName (∃ T, GlobalInvExt commit_test_ru T extract γmstate γmlin γmpost γmname γl clients) -∗
+    inv KVS_InvName (∃ T exec, GlobalInvExt commit_test_ru T extract γmstate γmlin γmpost γmname γl clients exec) -∗
     @init_client_proxy_spec _ _ _ _ lib res -∗
     @init_client_proxy_spec _ _ _ _ (KVS_wrapped_api lib) (wrapped_resources γmstate γmlin γmpost γmname γl clients res).
   Proof.
@@ -85,7 +85,7 @@ Section trace_proof.
     rewrite /TC_init_client_proxy /KVS_wrapped_api /wrap_init_client_proxy.
     wp_pures.
     wp_bind (ast.Fresh _).
-    iInv "HinvExt" as ">[%T [%t [%lt [%exec (Htr_is & HOwnLin & %HlinOf & %Hno_empty & %Hex 
+    iInv "HinvExt" as ">[%T [%exec [%t [%lt (Htr_is & HOwnLin & %HlinOf & %Hno_empty & %Hex 
       & %Hvalid_trans & %Hvalid_seq & %Hbased & %Hvalid_exec & Hstate_res & Hlin_res & Hpost_res)]]]]" "Hclose".
     wp_apply (aneris_wp_fresh with "[$Htr_inv $Htr_is]").
     {
@@ -125,7 +125,7 @@ Section trace_proof.
     iMod ("Hclose" with "[Htr_is HOwnLin Hlin_res Hpost_res Hstate_res]").
     {
       iNext.
-      iExists T, (t ++ [(#tag1, init_pre_emit_event)%V]), lt, exec.
+      iExists T, exec, (t ++ [(#tag1, init_pre_emit_event)%V]), lt.
       iFrame.
       iSplitR; last set_solver.
       iPureIntro.
@@ -141,7 +141,7 @@ Section trace_proof.
     wp_bind (ast.Emit _).
     rewrite /init_post_emit_event.
     wp_pures.
-    iInv "HinvExt" as ">[%T' [%t' [%lt' [%exec' (Htr_is' & HOwnLin' & %HlinOf' & %Hno_empty' & %Hex' 
+    iInv "HinvExt" as ">[%T' [%exec' [%t' [%lt' (Htr_is' & HOwnLin' & %HlinOf' & %Hno_empty' & %Hex' 
       & %Hvalid_trans' & %Hvalid_seq' & %Hbased' & %Hvalid_exec' & Hstate_res' & Hlin_res' & Hpost_res')]]]]" "Hclose'".
     iMod (own_lin_add _ _ (#tag1, (c, #"InLin"))%V with "[$HOwnLin']") as "HOwnLin'".
     iPoseProof (trace_hist_trace_is_prefix with "[$Htr_is'][$Htr_hist]") as "%Hprefix".
@@ -239,8 +239,8 @@ Section trace_proof.
       Hghost_map_mstate Hghost_map_m Hghost_elems_m Hlin_res' Hpost_res']").
     {
       iNext.
-      iExists T', (t' ++ [(#tag1, (c, #"InPost"))%V]), 
-        (lt' ++ [(#tag1, (c, #"InLin"))%V]), exec'.
+      iExists T', exec', (t' ++ [(#tag1, (c, #"InPost"))%V]), 
+        (lt' ++ [(#tag1, (c, #"InLin"))%V]).
       iFrame.
       do 2 (iSplit; first by iPureIntro).
       iSplit; first iPureIntro.
@@ -329,7 +329,7 @@ Section trace_proof.
   (lib : KVS_transaction_api) : 
     ⌜KVS_InvName = nroot .@ "kvs_inv"⌝ -∗
     trace_inv trace_inv_name valid_trace_ru -∗
-    inv KVS_InvName (∃ T, GlobalInvExt commit_test_ru T extract γmstate γmlin γmpost γmname γl clients) -∗
+    inv KVS_InvName (∃ T exec, GlobalInvExt commit_test_ru T extract γmstate γmlin γmpost γmname γl clients exec) -∗
     @read_spec _ _ _ _ lib res -∗
     @read_spec _ _ _ _ (KVS_wrapped_api lib) (wrapped_resources γmstate γmlin γmpost γmname γl clients res).
   Proof.
@@ -342,7 +342,7 @@ Section trace_proof.
     wp_bind (ast.Fresh _).
     rewrite /read_pre_emit_event.
     wp_pures.
-    iInv "HinvExt" as ">[%T [%t [%lt [%exec
+    iInv "HinvExt" as ">[%T [%exec [%t [%lt 
       (Htr_is & HOwnLin & %HlinOf & %Hno_empty & %Hex & %Hvalid_trans & %Hvalid_seq 
        & %Hbased & %Hvalid_exec & Hstate_res & Hlin_res & Hpost_res)]]]]" "Hclose".
     wp_apply (aneris_wp_fresh with "[$Htr_inv $Htr_is]").
@@ -382,7 +382,7 @@ Section trace_proof.
     iMod ("Hclose" with "[Htr_is HOwnLin Hstate_res Hlin_res Hpost_res]").
     {
       iNext.
-      iExists T, (t ++ [(#tag1, (c, #"RdPre"))%V]), lt, exec.
+      iExists T, exec, (t ++ [(#tag1, (c, #"RdPre"))%V]), lt.
       iFrame.
       iSplitR; last set_solver.
       iPureIntro.
@@ -403,7 +403,7 @@ Section trace_proof.
     iFrame.
     iNext.
     iIntros (wo) "(Hkey_c & Hkey)".
-    iInv "HinvExt" as ">[%T' [%t' [%lt' [%exec'
+    iInv "HinvExt" as ">[%T' [%exec' [%t' [%lt' 
       (Htr_is' & HOwnLin' & %HlinOf' & %Hno_empty' & %Hex' & %Hvalid_trans' & 
       %Hbased' & %Hvalid_exec' & %Hvalid_seq' & HstateRes' & Hlin_res' & Hpost_res')]]]]" "Hclose'".
     iMod (own_lin_add _ _ (#tag1, (c, (#"RdLin", (#k, $wo))))%V with "[$HOwnLin']") as "HOwnLin'".
@@ -531,7 +531,7 @@ Section trace_proof.
         op ∈ trans ∧ (λ op, last trans = Some op ∧ connOfOp op = c ∧ isCmOp op = false) op) trans)) 
           as [(trans & Htrans_in & Hop)|Hdec].
       - destruct (elem_of_list_split _ _ Htrans_in) as (T1 & T2 & ->).
-        iExists (T1 ++ (trans ++ [Rd (tag1, c) k wo]) :: T2), t', (lt' ++ [(#tag1, (c, (#"RdLin", (#k, $ wo))))%V]), exec'.
+        iExists (T1 ++ (trans ++ [Rd (tag1, c) k wo]) :: T2), exec', t', (lt' ++ [(#tag1, (c, (#"RdLin", (#k, $ wo))))%V]).
         iFrame.
         iSplit.
         + iPureIntro.
@@ -640,7 +640,7 @@ Section trace_proof.
                               exists e.
                               split_and!; try done.
                               apply elem_of_app; eauto.
-      - iExists (T' ++ [[Rd (tag1, c) k wo]]), t', (lt' ++ [(#tag1, (c, (#"RdLin", (#k, $ wo))))%V]), exec'.
+      - iExists (T' ++ [[Rd (tag1, c) k wo]]), exec', t', (lt' ++ [(#tag1, (c, (#"RdLin", (#k, $ wo))))%V]).
         iFrame.
         iSplit.
         + iPureIntro.
@@ -720,7 +720,7 @@ Section trace_proof.
     rewrite /read_post_emit_event.
     wp_pures.
     wp_bind (Emit _).
-    iInv "HinvExt" as ">[%T'' [%t'' [%lt'' [%exec''
+    iInv "HinvExt" as ">[%T'' [%exec'' [%t'' [%lt'' 
       (Htr_is'' & HOwnLin'' & %HlinOf'' & %Hno_empty'' & %Hex'' & %Hvalid_trans'' & 
       %Hbased'' & %Hvalid_exec'' & %Hvalid_seq'' & HstateRes'' & Hlin_res'' & Hpost_res'')]]]]" "Hclose''".
     iDestruct (own_lin_prefix with "[$HOwnLin'' $HOwnLinHist']") 
@@ -755,7 +755,7 @@ Section trace_proof.
     iMod ("Hclose''" with "[Htr_is'' HOwnLin'' HstateRes'' Hlin_res'' Hpost_res'']").
     {
       iModIntro.
-      iExists T'', (t'' ++ [_]), lt'', exec''.
+      iExists T'', exec'', (t'' ++ [_]), lt''.
       iFrame.
       iSplitR; last set_solver.
       iPureIntro.
@@ -773,7 +773,7 @@ Section trace_proof.
   (lib : KVS_transaction_api) : 
     ⌜KVS_InvName = nroot .@ "kvs_inv"⌝ -∗
     trace_inv trace_inv_name valid_trace_ru -∗
-    inv KVS_InvName (∃ T, GlobalInvExt commit_test_ru T extract γmstate γmlin γmpost γmname γl clients) -∗
+    inv KVS_InvName (∃ T exec, GlobalInvExt commit_test_ru T extract γmstate γmlin γmpost γmname γl clients exec) -∗
     @write_spec _ _ _ _ lib res -∗
     @write_spec _ _ _ _ (KVS_wrapped_api lib) (wrapped_resources γmstate γmlin γmpost γmname γl clients res).
   Proof.
@@ -786,7 +786,7 @@ Section trace_proof.
     wp_bind (ast.Fresh _).
     rewrite /write_pre_emit_event.
     wp_pures.
-    iInv "HinvExt" as ">[%T [%t [%lt [%exec 
+    iInv "HinvExt" as ">[%T [%exec [%t [%lt  
       (Htr_is & HOwnLin & %HlinOf & %Hno_empty & %Hex & %Hvalid_trans & %Hvalid_seq &
       %Hbased & %Hvalid_exec & Hstate_res & Hlin_res & Hpost_res)]]]]" "Hclose".
     wp_apply (aneris_wp_fresh with "[$Htr_inv $Htr_is]").
@@ -826,7 +826,7 @@ Section trace_proof.
     iMod ("Hclose" with "[Htr_is HOwnLin Hstate_res Hlin_res Hpost_res]").
     {
       iNext.
-      iExists T, (t ++ [(#tag1, (c, #"WrPre"))%V]), lt, exec.
+      iExists T, exec, (t ++ [(#tag1, (c, #"WrPre"))%V]), lt.
       iFrame.
       iSplitR; last set_solver.
       iPureIntro.
@@ -847,7 +847,7 @@ Section trace_proof.
     iFrame.
     iNext.
     iIntros "(Hkey_c & Hkey)".
-    iInv "HinvExt" as ">[%T' [%t' [%lt' [%exec'
+    iInv "HinvExt" as ">[%T' [%exec' [%t' [%lt' 
       (Htr_is' & HOwnLin' & %HlinOf' & %Hno_empty' & %Hex' & %Hvalid_trans' & 
       %Hbased' & %Hvalid_exec' & %Hvalid_seq' & HstateRes' & Hlin_res' & Hpost_res')]]]]" "Hclose'".
     iMod (own_lin_add _ _ (#tag1, (c, (#"WrLin", (#k, v))))%V with "[$HOwnLin']") as "HOwnLin'".
@@ -920,7 +920,7 @@ Section trace_proof.
         op ∈ trans ∧ (λ op, last trans = Some op ∧ connOfOp op = c ∧ isCmOp op = false) op) trans)) 
           as [(trans & Htrans_in & Hop)|Hdec].
       - destruct (elem_of_list_split _ _ Htrans_in) as (T1 & T2 & ->).
-        iExists (T1 ++ (trans ++ [Wr (tag1, c) k v]) :: T2), t', (lt' ++ [(#tag1, (c, (#"WrLin", (#k, v))))%V]), exec'.
+        iExists (T1 ++ (trans ++ [Wr (tag1, c) k v]) :: T2), exec', t', (lt' ++ [(#tag1, (c, (#"WrLin", (#k, v))))%V]).
         iFrame.
         iSplit.
         + iPureIntro.
@@ -967,7 +967,7 @@ Section trace_proof.
                             exists e.
                             split_and!; try done.
                             apply elem_of_app; eauto. 
-      - iExists (T' ++ [[Wr (tag1, c) k v]]), t', (lt' ++ [(#tag1, (c, (#"WrLin", (#k, v))))%V]), exec'.
+      - iExists (T' ++ [[Wr (tag1, c) k v]]), exec', t', (lt' ++ [(#tag1, (c, (#"WrLin", (#k, v))))%V]).
         iFrame.
         iSplit.
         + iPureIntro.
@@ -1042,7 +1042,7 @@ Section trace_proof.
     iModIntro.
     rewrite /write_post_emit_event.
     wp_pures.
-    iInv "HinvExt" as ">[%T'' [%t'' [%lt'' [%exec''
+    iInv "HinvExt" as ">[%T'' [%exec'' [%t'' [%lt'' 
       (Htr_is'' & HOwnLin'' & %HlinOf'' & %Hno_empty'' & %Hex'' & %Hvalid_trans'' & 
       %Hbased'' & %Hvalid_exec'' & %Hvalid_seq'' & HstateRes'' & Hlin_res'' & Hpost_res'')]]]]" "Hclose''".
     iDestruct (own_lin_prefix with "[$HOwnLin'' $HOwnLinHist']") 
@@ -1076,7 +1076,7 @@ Section trace_proof.
     iMod ("Hclose''" with "[Htr_is'' HOwnLin'' HstateRes'' Hlin_res'' Hpost_res'']").
     {
       iModIntro.
-      iExists T'', (t'' ++ [(#tag1, (c, (#"WrPost", (#k, v))))%V]), lt'', exec''.
+      iExists T'', exec'', (t'' ++ [(#tag1, (c, (#"WrPost", (#k, v))))%V]), lt''.
       iFrame.
       iSplitR; last set_solver.
       iPureIntro.
@@ -1091,7 +1091,7 @@ Section trace_proof.
   (lib : KVS_transaction_api) : 
     ⌜KVS_InvName = nroot .@ "kvs_inv"⌝ -∗
     trace_inv trace_inv_name valid_trace_ru -∗
-    inv KVS_InvName (∃ T, GlobalInvExt commit_test_ru T extract γmstate γmlin γmpost γmname γl clients) -∗
+    inv KVS_InvName (∃ T exec, GlobalInvExt commit_test_ru T extract γmstate γmlin γmpost γmname γl clients exec) -∗
     @start_spec _ _ _ _ lib res -∗
     @start_spec _ _ _ _ (KVS_wrapped_api lib) (wrapped_resources γmstate γmlin γmpost γmname γl clients res).
   Proof.
@@ -1104,7 +1104,7 @@ Section trace_proof.
     wp_bind (ast.Fresh _).
     rewrite /start_pre_emit_event.
     wp_pures.
-    iInv "HinvExt" as ">[%T [%t [%lt [%exec
+    iInv "HinvExt" as ">[%T [%exec [%t [%lt 
       (Htr_is & HOwnLin & %HlinOf & %Hno_empty & %Hex & %Hvalid_trans & %Hvalid_seq &
       %Hbased & %Hvalid_exec & Hstate_res & Hlin_res & Hpost_res)]]]]" "Hclose".
     wp_apply (aneris_wp_fresh with "[$Htr_inv $Htr_is]").
@@ -1144,7 +1144,7 @@ Section trace_proof.
     iMod ("Hclose" with "[Htr_is HOwnLin Hstate_res Hlin_res Hpost_res]").
     {
       iNext.
-      iExists T, (t ++ [(#tag1, (c, #"StPre"))%V]), lt, exec.
+      iExists T, exec, (t ++ [(#tag1, (c, #"StPre"))%V]), lt.
       iFrame.
       iSplitR; last set_solver.
       iPureIntro.
@@ -1165,7 +1165,7 @@ Section trace_proof.
     iFrame.
     iModIntro.
     iIntros "(Hconn_state & Hkeys1 & Hkeys_conn)".
-    iInv "HinvExt" as ">[%T' [%t' [%lt' [%exec' 
+    iInv "HinvExt" as ">[%T' [%exec' [%t' [%lt' 
       (Htr_is' & HOwnLin' & %HlinOf' & %Hno_empty' & %Hex' & %Hvalid_trans' & 
       %Hbased' & %Hvalid_exec' & %Hvalid_seq' & HstateRes' & Hlin_res' & Hpost_res')]]]]" "Hclose'".
     simpl; rewrite /trace_state_resources.
@@ -1262,7 +1262,7 @@ Section trace_proof.
       Hghost_map_mstate' Hkeys_conn_res2 Hlin_res' Hpost_res' Hdisj_trace_res]").
     {
       iModIntro.
-      iExists T', t', (lt' ++ [(#tag1, (c, #"StLin"))%V]), exec'.
+      iExists T', exec', t', (lt' ++ [(#tag1, (c, #"StLin"))%V]).
       iFrame.
       iSplitR.
       {
@@ -1395,7 +1395,7 @@ Section trace_proof.
     iModIntro.
     rewrite /start_post_emit_event.
     wp_pures.
-    iInv "HinvExt" as ">[%T'' [%t'' [%lt'' [%exec''
+    iInv "HinvExt" as ">[%T'' [%exec'' [%t'' [%lt''
       (Htr_is'' & HOwnLin'' & %HlinOf'' & %Hno_empty'' & %Hex'' & %Hvalid_trans'' & 
       %Hbased'' & %Hvalid_exec'' & %Hvalid_seq'' & HstateRes'' & Hlin_res'' & Hpost_res'')]]]]" "Hclose''".
     iDestruct (own_lin_prefix with "[$HOwnLin'' $HOwnLinHist']") 
@@ -1429,7 +1429,7 @@ Section trace_proof.
     iMod ("Hclose''" with "[Htr_is'' HOwnLin'' HstateRes'' Hlin_res'' Hpost_res'']").
     {
       iModIntro.
-      iExists T'', (t'' ++ [(#tag1, (c, #"StPost"))%V]), lt'', exec''.
+      iExists T'', exec'', (t'' ++ [(#tag1, (c, #"StPost"))%V]), lt''.
       iFrame.
       iSplitR; last set_solver.
       iPureIntro.
@@ -1444,7 +1444,7 @@ Section trace_proof.
   (lib : KVS_transaction_api) : 
     ⌜KVS_InvName = nroot .@ "kvs_inv"⌝ -∗
     trace_inv trace_inv_name valid_trace_ru -∗
-    inv KVS_InvName (∃ T, GlobalInvExt commit_test_ru T extract γmstate γmlin γmpost γmname γl clients) -∗
+    inv KVS_InvName (∃ T exec, GlobalInvExt commit_test_ru T extract γmstate γmlin γmpost γmname γl clients exec) -∗
     @commit_spec _ _ _ _ lib res -∗
     @commit_spec _ _ _ _ (KVS_wrapped_api lib) (wrapped_resources γmstate γmlin γmpost γmname γl clients res).
   Proof.
@@ -1457,7 +1457,7 @@ Section trace_proof.
     wp_bind (ast.Fresh _).
     rewrite /commit_pre_emit_event.
     wp_pures.
-    iInv "HinvExt" as ">[%T [%t [%lt [%exec
+    iInv "HinvExt" as ">[%T [%exec [%t [%lt 
       (Htr_is & HOwnLin & %HlinOf & %Hno_empty & %Hex & %Hvalid_trans & %Hvalid_seq &
       %Hbased & %Hvalid_exec & Hstate_res & Hlin_res & Hpost_res)]]]]" "Hclose".
     wp_apply (aneris_wp_fresh with "[$Htr_inv $Htr_is]").
@@ -1497,7 +1497,7 @@ Section trace_proof.
     iMod ("Hclose" with "[Htr_is HOwnLin Hstate_res Hlin_res Hpost_res]").
     {
       iNext.
-      iExists T, (t ++ [(#tag1, (c, #"CmPre"))%V]), lt, exec.
+      iExists T, exec, (t ++ [(#tag1, (c, #"CmPre"))%V]), lt.
       iFrame.
       iSplitR; last set_solver.
       iPureIntro.
@@ -1529,7 +1529,7 @@ Section trace_proof.
     }
     iModIntro.
     iIntros (b) "(Hstate & Hkeys1)".
-    iInv "HinvExt" as ">[%T' [%t' [%lt' [%exec'
+    iInv "HinvExt" as ">[%T' [%exec' [%t' [%lt' 
       (Htr_is' & HOwnLin' & %HlinOf' & %Hno_empty' & %Hex' & %Hvalid_trans' & 
       %Hbased' & %Hvalid_exec' & %Hvalid_seq' & HstateRes' & Hlin_res' & Hpost_res')]]]]" "Hclose'".
     iMod (own_lin_add _ _ (#tag1, (c, (#"CmLin", #b)))%V with "[$HOwnLin']") as "HOwnLin'".
@@ -1616,8 +1616,8 @@ Section trace_proof.
           apply app_eq_nil in Hfalse.
           set_solver.
         }
-        iExists (T1 ++ (trans ++ [Cm (tag1, c) b]) :: T2), t', 
-          (lt' ++ [(#tag1, (c, (#"CmLin", #b)))%V]), exec''.
+        iExists (T1 ++ (trans ++ [Cm (tag1, c) b]) :: T2), exec'', t', 
+          (lt' ++ [(#tag1, (c, (#"CmLin", #b)))%V]).
         iFrame.
         iSplit.
         + iPureIntro.
@@ -1669,7 +1669,7 @@ Section trace_proof.
         }
         destruct (exists_execution (T' ++ [[Cm (tag1, c) b]]))
           as (exec'' & Hbased'' & Hvalid_exec''); first set_solver; try done.
-        iExists (T' ++ [[Cm (tag1, c) b]]), t', (lt' ++ [(#tag1, (c, (#"CmLin", #b)))%V]), exec''.
+        iExists (T' ++ [[Cm (tag1, c) b]]), exec'', t', (lt' ++ [(#tag1, (c, (#"CmLin", #b)))%V]).
         iFrame.
         iSplit.
         + iPureIntro.
@@ -1716,7 +1716,7 @@ Section trace_proof.
     rewrite /commit_post_emit_event.
     wp_pures.
     wp_bind (Emit _).
-    iInv "HinvExt" as ">[%T'' [%t'' [%lt'' [%exec''
+    iInv "HinvExt" as ">[%T'' [%exec'' [%t'' [%lt'' 
       (Htr_is'' & HOwnLin'' & %HlinOf'' & %Hno_empty'' & %Hex'' & %Hvalid_trans'' & 
       %Hbased'' & %Hvalid_exec'' & %Hvalid_seq'' & HstateRes'' & Hlin_res'' & Hpost_res'')]]]]" "Hclose''".
     iDestruct (own_lin_prefix with "[$HOwnLin'' $HOwnLinHist']") 
@@ -1750,7 +1750,7 @@ Section trace_proof.
     iMod ("Hclose''" with "[Htr_is'' HOwnLin'' HstateRes'' Hlin_res'' Hpost_res'']").
     {
       iModIntro.
-      iExists T'', (t'' ++ [(#tag1, (c, (#"CmPost", #b)))%V]), lt'', exec''.
+      iExists T'', exec'', (t'' ++ [(#tag1, (c, (#"CmPost", #b)))%V]), lt''.
       iFrame.
       iSplitR; last set_solver.
       iPureIntro.
@@ -1785,11 +1785,11 @@ Section trace_proof.
       by apply gmap_of_trace_valid.
     }
     iDestruct "Hltrace" as "[Hltrace Hlhist]".
-    iMod (inv_alloc KVS_InvName ⊤ (∃ T, GlobalInvExt commit_test_ru T extract γmstate γmlin γmpost γmname γl clients) with 
+    iMod (inv_alloc KVS_InvName ⊤ (∃ T exec, GlobalInvExt commit_test_ru T extract γmstate γmlin γmpost γmname γl clients exec) with 
       "[Htr Hghost_map_mstate Hghost_map_mlin Hghost_map_mpost Hghost_map_mname Hltrace Hlhist]") as "#HinvExt".
     {
       iNext.
-      iExists [], [], [], [([], ∅)].
+      iExists [], [([], ∅)], [], [].
       iFrame.
       simpl.
       iSplitR.
